examples/new_stack/NewClientImp0proof.v
@@ -1,0 +1,79 @@
+Require Import HoareDef SimModSem.
+Require Import Coqlib.
+Require Import Universe.
+Require Import Skeleton.
+Require Import PCM.
+Require Import ModSem Behavior.
+Require Import Relation_Definitions.
+
+(*** TODO: export these in Coqlib or Universe ***)
+Require Import Relation_Operators.
+Require Import RelationPairs.
+From ITree Require Import
+     Events.MapDefault.
+From ExtLib Require Import
+     Core.RelDec
+     Structures.Maps
+     Data.Map.FMapAList.
+Require Import TODOYJ.
+Require Import HTactics Logic IPM.
+Require Import OpenDef.
+Require Import Mem1 MemOpen STB.
+
+Require Import Imp.
+Require Import ImpNotations.
+Require Import ImpProofs.
+
+Require Import NewClient0 NewClientImp.
+
+Set Implicit Arguments.
+
+Local Open Scope nat_scope.
+
+Section SIMMODSEM.
+
+  Import ImpNotations.
+
+  Context `{Σ: GRA.t}.
+
+  Let W: Type := Any.t * Any.t.
+
+  Let wf: unit -> W -> Prop :=
+    fun _ '(mrps_src0, mrps_tgt0) =>
+      (<<SRC: mrps_src0 = tt↑>>) /\
+      (<<TGT: mrps_tgt0 = tt↑>>)
+  .
+
+  Theorem correct:
+    forall ge, ModSemPair.sim NewClient0.ClientSem (NewClientImp.ClientSem ge).
+  Proof.
+    Local Transparent syscalls.
+    econstructor 1 with (wf:=wf) (le:=top2); et; ss.
+    econs; ss.
+    { init.
+      unfold getintF, getint.
+      steps.
+      rewrite unfold_eval_imp. steps.
+      des_ifs.
+      2:{ exfalso; apply n. solve_NoDup. }
+      imp_steps.
+      gstep. econs; ss. i. exists 100. imp_steps.
+      red. esplits; et.
+    }
+    econs; ss.
+    { init.
+      steps.
+      unfold putintF, putint.
+      steps.
+      rewrite unfold_eval_imp. steps.
+      des_ifs.
+      2:{ exfalso; apply n. solve_NoDup. }
+      imp_steps.
+      gstep. econs; ss. i. exists 100. imp_steps.
+      red. esplits; et.
+    }
+    Local Opaque syscalls.
+    Unshelve. all: ss.
+  Qed.
+
+End SIMMODSEM.
